Security/Polynomial/SaberPolyQuotient/MLWRGamesROMSecurity.ec
@@ -1,0 +1,194 @@
+pragma Goals:printall.
+
+(*
+----------------------------------- 
+ Require/Import EasyCrypt Theories
+-----------------------------------
+*)
+(* --- Built-in --- *)
+require import AllCore Distr DBool ZModP IntDiv StdOrder PROM.
+require (*--*) Matrix PKE.
+
+(* --- Local --- *)
+require import SaberRqPreliminaries.
+(*---*) import Rq Rp Rppq R2t R2.
+(*---*) import Mat_Rq Mat_Rp.
+
+(*
+----------------------------------- 
+ ROM
+-----------------------------------
+*)
+
+clone import FullRO with
+  type in_t <- seed,
+  type out_t <- Rq_mat,
+  op dout <- (fun (sd : seed) => dRq_mat).
+
+(*
+--------------------------------
+ Adversary Prototypes
+--------------------------------
+*)
+module type Adv_MLWR = {
+  proc guess(_A : Rq_mat, b : Rp_vec) : bool
+}.
+
+module type Adv_GMLWR_RO(Gen : RO) = {
+   proc guess(sd : seed, b : Rp_vec) : bool { Gen.get }
+}.
+
+module type Adv_XMLWR_RO(Gen : RO) = {
+   proc guess(sd : seed, b : Rp_vec, a : Rq_vec, d : Rp) : bool { Gen.get }
+}.
+
+(*
+--------------------------------
+ Games
+--------------------------------
+*)
+
+(* --- Original (transposed) MLWR Game --- *)
+module MLWR(A : Adv_MLWR) = {
+    proc main(u : bool) : bool = {
+       var u' : bool;
+       var _A : Rq_mat;
+       var s : Rq_vec;
+       var b : Rp_vec;
+
+       _A <$ dRq_mat;
+       s <$ dsmallRq_vec;
+       
+       if (u) {
+          b <$ dRp_vec; 
+       } else {
+          b <- scale_vec_Rq_Rp (_A *^ s + h);
+       }
+       
+       u' <@ A.guess(_A, b);
+
+       return u';
+    }
+}.
+
+(* --- LWR-Related Games in ROM --- *)
+module GMLWR_RO(A : Adv_GMLWR_RO) = {
+   module A = A(RO)
+
+   proc main(u : bool) : bool = {
+      var u' : bool;
+      var sd : seed;
+      var _A : Rq_mat;
+      var s : Rq_vec;
+      var b : Rp_vec;
+
+      RO.init();
+
+      sd <$ dseed;
+      _A <@ RO.get(sd);
+      s <$ dsmallRq_vec;
+      
+      if (u) {
+         b <$ dRp_vec;
+      } else {
+         b <- scale_vec_Rq_Rp (_A *^ s + h);
+      }
+      
+      u' <@ A.guess(sd, b);
+      
+      return u';
+   }
+}.
+
+module XMLWR_RO(A : Adv_XMLWR_RO) = {
+   module A = A(RO)
+
+   proc main(u : bool) : bool = {
+      var u' : bool;
+      var sd : seed;
+      var _A : Rq_mat;
+      var s : Rq_vec;
+      var b : Rp_vec;
+      var a : Rq_vec;
+      var d : Rp;
+
+      RO.init();
+
+      sd <$ dseed;
+      _A <- RO.get(sd);
+      s <$ dsmallRq_vec;
+      
+      if (u) {
+         b <$ dRp_vec;
+      } else {
+         b <- scale_vec_Rq_Rp ((trmx _A) *^ s + h);
+      }
+      
+      a <$ dRq_vec;
+
+      if (u) {
+         d <$ dRp;
+      } else {
+         d <- scale_Rq_Rp ((dotp a s) + h1);
+      }
+    
+      u' <@ A.guess(sd, b, a, d);
+      
+      return u';
+   }
+}.
+
+(*
+--------------------------------
+ Adversaries
+--------------------------------
+*)
+module AGM(AG : Adv_GMLWR_RO) : Adv_MLWR = {
+   module AG = AG(RO)
+
+   proc guess(_A : Rq_mat, b : Rp_vec) : bool = {
+      var u' : bool;
+      var sd : seed;
+
+      RO.init();
+
+      sd <$ dseed;
+
+      RO.set(sd, _A);
+
+      u' <@ AG.guess(sd, b);
+
+      return u';
+   } 
+}.
+
+
+
+(*
+--------------------------------
+ Reductions
+--------------------------------
+*)
+
+lemma GMLWR_RO_to_MLWR &m (A <: Adv_GMLWR_RO{RO}) :
+  `| Pr[GMLWR_RO(A).main(true) @ &m : res] - Pr[GMLWR_RO(A).main(false) @ &m : res] |
+   =
+  `| Pr[MLWR( AGM(A) ).main(true) @ &m : res] - Pr[MLWR( AGM(A) ).main(false) @ &m : res] |.
+proof.
+  have ->: Pr[GMLWR_RO(A).main(true) @ &m : res] =  Pr[MLWR( AGM(A) ).main(true) @ &m : res].
+   byequiv => //.
+   proc; inline *.
+   rcondt {1} 8; 2: rcondt {2} 3; first 2 auto.
+   rcondt {1} 5; first auto; progress; smt.
+   swap {1} [7..8] -2; swap {1} [4..6] -2.
+   by wp; call (_ : ={RO.m}); 1: proc; auto.
+  have -> //: Pr[GMLWR_RO(A).main(false) @ &m : res] =  Pr[MLWR( AGM(A) ).main(false) @ &m : res].
+   byequiv => //.
+   proc; inline *.
+   rcondf {1} 8; 2: rcondf {2} 3; first 2 auto.
+   rcondt {1} 5; first auto; progress; smt.
+   swap {1} 4 -3; swap {1} 7 -5. 
+   wp; call (_ : ={RO.m}); 1: proc; auto.
+   progress; smt.
+qed.  
+
